concurrency/DryMachineSource.v
@@ -28,7 +28,15 @@ Require Import concurrency.erased_machine.
 Require Import veric.Clight_new.
 Require Import veric.Clightnew_coop.
 Require Import sepcomp.event_semantics.
+Require Import veric.Clight_sim.
 Require Import concurrency.ClightSemantincsForMachines.
+
+(*SSReflect*)
+From mathcomp.ssreflect Require Import ssreflect ssrfun ssrbool ssrnat eqtype seq.
+Require Import Coq.ZArith.ZArith.
+Require Import PreOmega.
+Require Import concurrency.ssromega. (*omega in ssrnat *)
+Set Bullet Behavior "Strict Subproofs".
 
 Import Concur threadPool.
 
@@ -68,5 +76,234 @@ Module THE_DRY_MACHINE_SOURCE.
      
   End DMS.
   Module DryMachineLemmas := ThreadPoolWF SEM DMS.
+
+  Module FiniteBranching.
+    
+  (** *Finite Branching*)
+    (* Probably need to assume something about memory.
+     Such as:
+     1. Next block increases at most by one
+     2. semantics is deterministic, so we know all possible changes to memory.
+     3. it's finitely branching *)
+  
+  Lemma finite_branching: forall ds ge,
+          safety.finite_on_x
+            (@safety.possible_image
+               DMS.DryConc.new_state
+               DMS.DryConc.Sch
+               (fun x y x' => exists y', (DMS.DryConc.new_step ge x y x' y'))
+               DMS.DryConc.new_valid ds).
+  Proof.
+    move=> [] [] tr dm m  prog.
+    rewrite /safety.finite_on_x /safety.possible_image /=.
+    rewrite /DMS.DryConc.new_step /DMS.DryConc.new_valid /=.
+    rewrite /DMS.DryConc.valid /DMS.DryConc.correct_schedule.
+    rewrite /DMS.DryConc.unique_Krun /DMS.DryMachine.ThreadPool.containsThread.
+    rewrite /DMS.DryConc.mk_ostate.
+    (*First check if it's mem_compatible. If not, it can't step! *)
+    pose (mem_compat_dec:=
+              DMS.DryMachine.mem_compatible dm m).
+    destruct (Classical_Prop.classic mem_compat_dec) as [Hcmpt|NHcmpt].
+    Focus 2. (*it can't step! *)
+    { 
+    exists 1%nat, (fun _ => (tr, dm, m)).
+    move => x y [] val [] y' stp.
+    inversion stp; subst.
+    - exists O; split.
+      + compute; reflexivity.
+      + destruct x as [[ ? ?] ?]; reflexivity.
+    - inversion H; destruct x as [[a b] c]; simpl in *; subst;
+      try solve [exfalso; apply NHcmpt; exact Hcmpt].
+      (*only the schedule fail is left*)
+       exists O; split.
+      + compute; reflexivity.
+      + reflexivity.
+    } Unfocus.
+    
+    (*Second check if any thread is running*)
+    pose (running_dec:=
+              exists i q cnti,
+                @DMS.DryMachine.ThreadPool.getThreadC i dm cnti = Krun q /\
+          ~ DMS.DryMachine.threadHalted cnti ).
+    destruct (Classical_Prop.classic running_dec) as [H|H]; move: H.
+    { (*First case were something is running*)
+      move => [] i [] q [] cnti [] is_running not_halted.
+      (*If the schedule is empty, it's halted so the same state *)
+      pose (st0 := (tr,dm,m)).
+      (* Otherwise, make a fake schedule, standing in for the real one *)
+      pose (sch0:= i::nil).
+      (*Step suspending would go to: *)
+      pose (st1 := (tr,DMS.DryMachine.ThreadPool.updThreadC cnti (Kblocked q),m)).
+      (*Otherwise it will take a step*)
+      pose (m1:= restrPermMap (DMS.DryMachine.compat_th Hcmpt cnti).1).
+      pose (step_dec:=
+              exists c' m',
+                veric.Clight_new.cl_step prog q m1 c' m').
+      destruct (Classical_Prop.classic step_dec) as [steps | steps]; move: steps.
+      - move=> [] c' [] m' steps.
+        pose (st2 := (tr,
+                      DMS.DryMachine.ThreadPool.updThread
+                        cnti
+                        (Krun c')
+                        (getCurPerm m',
+                         (DMS.DryMachine.ThreadPool.getThreadR cnti).2)
+                      ,m')).
+        exists 4%nat.
+        exists (fun i => match i with
+                 | O => st0
+                 | 1%nat => st1
+                 | _ => st2
+                         end).
+        move => x y [] VAL [] y' steps2.
+        inversion steps2; subst.
+        + (* if halted *)
+          exists O; split.
+          * compute; reflexivity.
+          * destruct x as [[? ?] ?]; reflexivity.
+        + (*its a machine step*)
+          simpl in VAL.
+          destruct (SCH.schedPeek y ) eqn:PEEK.
+          Focus 2. (*Halted*)
+          { simpl in H.
+            inversion H; simpl in *; try subst y;
+            try congruence. (*All other steps will contradict hyp. PEEK*)
+          } Unfocus.
+          (*If not halted, the running thread is i*)
+          specialize (VAL _ _ _ is_running not_halted);
+            destruct (SCH.TID.eq_tid_dec); inversion VAL; subst t.
+          inversion H; (*Lets go through all possible steps*)
+            simpl in *; subst;
+          match goal with
+          | [ H: SCH.schedPeek ?Y = Some _ ,
+                 H': SCH.schedPeek ?Y = Some _  |- _ ] =>
+            rewrite H in H'; inversion H'; subst
+          end;
+          try ( inversion Htstep;
+                match goal with
+                | [ H: DMS.DryMachine.ThreadPool.getThreadC ?cnt1 = _ ,
+                       H': DMS.DryMachine.ThreadPool.getThreadC ?cnt2 = _  |- _ ] =>
+                  replace cnt2 with cnt1 in H' by apply proof_irrelevance;
+                    rewrite H in H'; inversion H'
+                end) .
+          * (*Thread step*)
+            subst.
+            apply ev_step_ax1 in Hcorestep.
+            move: Hcorestep.
+            rewrite /DMS.DryMachine.ThreadPool.SEM.Sem SEM.CLN_msem /= => steps'.
+            (*We use that CLight is deterministic: *)
+            Lemma CLight_Deterministic: forall ge c m c1 m1 c2 m2,
+                veric.Clight_new.cl_step ge c m c2 m2 ->
+                veric.Clight_new.cl_step ge c m c1 m1 ->
+                c1 = c2 /\ m1 = m2.
+                    
+            Admitted.
+            move: steps'.
+            replace Hcmpt0 with Hcmpt by apply proof_irrelevance;
+              replace Htid with cnti by apply proof_irrelevance .
+            move => steps'.
+            destruct (CLight_Deterministic _ _ _ _ _ _ _ steps steps').
+            exists 2%nat; split.
+            -- compute; reflexivity.
+            -- destruct x as [[? ?]?]; simpl in *; subst.
+               unfold st2; simpl.
+               replace Htid with cnti by apply proof_irrelevance.
+               reflexivity.
+          * (*suspend_step *)
+            exists 1%nat.
+            split.
+            -- compute; reflexivity.
+            -- destruct x as [[? ?]?]; simpl in *; subst.
+               unfold st1; simpl.
+               replace Htid with cnti by apply proof_irrelevance.
+               reflexivity.
+          * (*Halted*)
+            exfalso.
+            apply not_halted.
+            replace cnti with Htid by apply proof_irrelevance.
+            assumption.
+          * (*Schedule fail*)
+            exfalso.
+            apply Htid.
+            assumption.
+      - (*Other cases when can't step*)
+        exists 3%nat.
+        exists (fun i => match i with
+                 | O => st0
+                 | _ => st1
+                 end) => x y /=.
+        move => [] VAL [] y' steps2.
+        inversion steps2; subst.
+        + (* if halted *)
+          exists O; split.
+          * compute; reflexivity.
+          * destruct x as [[? ?] ?]; reflexivity.
+        + (*its a machine step*)
+          simpl in VAL.
+          destruct (SCH.schedPeek y) eqn:PEEK.
+          Focus 2. (*Halted*)
+          { simpl in H.
+            inversion H;
+            simpl in *; subst y;
+            simpl in *; try subst U;
+            try congruence. (*All other steps will contradict hyp. PEEK*)
+          } Unfocus.
+          (*If not halted, the running thread is i*)
+          specialize (VAL _ _ _ is_running not_halted);
+            destruct (SCH.TID.eq_tid_dec); inversion VAL; subst t.
+          subst.
+          inversion H; (*Lets go through all possible steps*)
+            simpl in *; try subst;
+          try match goal with
+          | [ H: SCH.schedPeek ?Y = Some _ ,
+                 H': SCH.schedPeek ?Y = Some _  |- _ ] =>
+            rewrite H in H'; inversion H'; subst
+          end; try subst;
+          try ( inversion Htstep;
+                match goal with
+                | [ H: DMS.DryMachine.ThreadPool.getThreadC ?cnt1 = _ ,
+                       H': DMS.DryMachine.ThreadPool.getThreadC ?cnt2 = _  |- _ ] =>
+                  replace cnt2 with cnt1 in H' by apply proof_irrelevance;
+                    rewrite H in H'; inversion H'
+                end) ;
+          try subst.
+          * (*Thread step*)
+            subst.
+            apply ev_step_ax1 in Hcorestep.
+            exfalso; apply steps.
+            rewrite /step_dec.
+            exists c', x.2.
+            unfold m1.
+            replace Hcmpt with Hcmpt0 by apply proof_irrelevance.
+            replace cnti with Htid by apply proof_irrelevance.
+            unfold DMS.DryMachine.ThreadPool.SEM.Sem in Hcorestep.
+            rewrite ClightSEM.CLN_msem in Hcorestep.
+            simpl in Hcorestep.
+            assumption.
+          * (*suspend step*)
+            simpl in *;
+            subst.
+            exists 1%nat; split.
+            -- compute; reflexivity.
+            -- destruct x as [[xa xb] xc]; simpl in *.
+               simpl.
+               replace ctn with cnti in Hms' by apply proof_irrelevance.
+               unfold st1.
+               rewrite Hms'.
+               subst.
+               reflexivity.
+          * exfalso; apply not_halted.
+            replace cnti with Htid by apply proof_irrelevance.
+            assumption.
+          * exfalso; apply Htid.
+            assumption.
+    }
+    { (*Second case when all threads are blocked, suspended or halted. *)
+    admit.
+    }
+    
+  Admitted.
+  
+  End FiniteBranching.
   
 End THE_DRY_MACHINE_SOURCE.
+
