concurrency/dry_machine.v
@@ -1236,6 +1236,7 @@ Module Concur.
           eauto. eauto. eauto.
   Admitted.
 
+
   End DryMachineShell.
   
 End Concur.
