concurrency/erasure_proof.v
@@ -1001,38 +1001,8 @@ Module Parching <: ErasureSig.
         rewrite C.
         f_equal.
       - (* THIS COULD BE A LEMMA*)
-        pose (IM:=(DryMachine.initial_machine pmap.1 c)); fold IM.
-        assert (isZ: forall i, DTP.containsThread IM i -> (i = 0)%N).
-        { rewrite /DryMachine.ThreadPool.containsThread /IM /=.
-          move => i; destruct i; first[reflexivity | intros HH; inversion HH].
-        }
-        assert (noLock: forall l rm, 
-                   DryMachine.ThreadPool.lockRes IM l = Some rm -> False).
-        { rewrite /DryMachine.ThreadPool.lockRes /IM /=.
-          move => l rm.
-          rewrite /DryMachine.ThreadPool.lockRes
-                  /DryMachine.initial_machine
-                  /empty_lset /= find_empty => HH.
-          inversion HH.
-          }
-
-        constructor.
-        + move => i j0 cnti cntj HH.
-          exfalso; apply HH.
-          move: cnti cntj => /isZ -> /isZ ->; reflexivity.
-        + move=> l1 l2 rm1 rm2 neq /noLock contra; inversion contra. 
-        + move => i l cnt rm /noLock contra; inversion contra.
-        + move=> i cnti; split.
-          * move => j0 cntj.
-            move: (cnti) (cntj) => cnti0 cntj0;
-              move: cnti cntj => /isZ Hi /isZ Hj.
-            subst.
-            eapply permCoh_empty'.
-          * move => l rm /noLock contra; inversion contra.
-        + move => l mr /noLock contra; inversion contra.
-        + move => b ofs.
-          rewrite / IM /= //.
-          
+        eapply initial_invariant0.
+        
       - apply MTCH_initial; assumption.
     Qed.
 
